Verified sortedInsert in UserDatabase

verification/UserDatabase.dfy
@@ -81,8 +81,7 @@ class UserDatabase {
 
     method doubleSize()
         modifies this, this.users, this.passwords
-        requires Valid(); ensures Valid()
-        requires users.Length == passwords.Length
+        requires Valid(); ensures Valid();
         ensures users.Length == passwords.Length
         ensures users.Length == old(users.Length) * 2
         ensures passwords.Length == old(passwords.Length) * 2
@@ -90,6 +89,8 @@ class UserDatabase {
         ensures users[..|old(users[..])|] == old(users[..])
         ensures old(passwords[..]) <= passwords[..]
         ensures passwords[..|old(passwords[..])|] == old(passwords[..])
+        ensures count == old(count)
+        ensures fresh(users) && fresh(passwords)
     {
         var newSize := users.Length * 2;
         
@@ -128,15 +129,84 @@ class UserDatabase {
             i := i + 1;
         }
         
-        var newUsersArr := seqToArrInt(newUsers);
+        var newUsersArr := seqToArrInt(newUsers); 
         var newPwdsArr := seqToArrStr(newPwds);
 
         users := newUsersArr;
         passwords := newPwdsArr;
-
     }
 
     // TODO sortedInsert(ID: int, pass: string)
+    method sortedInsert(newUserID: int, newUserPass: string)
+    modifies this, this.users, this.passwords, this`count; 
+    requires Valid(); ensures Valid();
+    requires users.Length > 0; 
+    ensures count == old(count) + 1;
+    ensures if old(count) == old(users.Length) 
+            then fresh(users) && users.Length == 2 * old(users.Length)
+            else users == old(users);
+    ensures if old(count) == old(users.Length) 
+            then fresh(passwords) && passwords.Length == 2 * old(passwords.Length) 
+            else passwords == old(passwords);
+    ensures exists index :: 0 <= index < count && (
+            (forall j :: 0 <= j < index ==> users[j] == old(users[j]) && passwords[j] == old(passwords[j])) &&
+            users[index] == newUserID && passwords[index] == newUserPass &&
+            (forall j :: index < j < count ==> users[j] == old(users[j-1]) && passwords[j] == old(passwords[j-1]))
+    );
+    {
+        if (count == users.Length) 
+        {
+            doubleSize();
+        }
+        assert count == old(count);
+        assert count == old(users.Length) ==> fresh(users) && fresh(passwords);
+        assert users.Length == if count == old(users.Length) then old(users.Length) * 2 else old(users.Length);
+        assert passwords.Length == users.Length;
+        assert forall k :: 0 <= k < count ==> users[k] == old(users[k]) && passwords[k] == old(passwords[k]);
+    
+        var i: int := 0; 
+        while (i < count && users[i] < newUserID) 
+        invariant 0 <= i <= count; 
+        invariant Sorted(0, count, users[..]);
+        invariant LTRange(users, 0, i, newUserID);
+        invariant forall k :: 0 <= k < count ==> users[k] == old(users[k]) && passwords[k] == old(passwords[k]);
+        {
+            i := i + 1; 
+        }
+
+        assert 0 <= i <= count < users.Length; 
+        assert count == old(count);
+        assert count == old(users.Length) ==> fresh(users) && fresh(passwords);
+        assert users.Length == if count == old(users.Length) then old(users.Length) * 2 else old(users.Length);
+        assert passwords.Length == users.Length;
+        assert LTRange(users, 0, i, newUserID);
+        assert GERange(users, i, count, newUserID);
+        assert users != null;
+
+
+        var j: int := count - 1; 
+        while (j >= i) 
+        invariant i - 1 <= j <= count - 1; 
+        invariant users != null;
+        invariant passwords != null;
+        invariant count == old(count); 
+        invariant if count == old(users.Length) then fresh(users) else users == old(users);
+        invariant if count == old(users.Length) then fresh(passwords) else passwords == old(passwords);
+        invariant users.Length == if count == old(users.Length) then 2 * old(users.Length) else old(users.Length);
+        invariant passwords.Length == users.Length;
+        invariant LTRange(users, 0, i, newUserID);
+        invariant forall k :: 0 <= k < j + 1 ==> users[k] == old(users[k]) && passwords[k] == old(passwords[k]);
+        invariant forall k :: j + 1 < k <= count ==> users[k] == old(users[k-1]) && passwords[k] == old(passwords[k-1]);
+        {
+            users[j+1] := users[j];
+            passwords[j+1] := passwords[j];
+            j := j - 1; 
+        }
+        count := count + 1; 
+        users[i] := newUserID;
+        passwords[i] := newUserPass;
+    }
+
 
     method getUsers() returns (userList: array<int>, passList: array<string>)
         requires Valid(); ensures Valid()
@@ -146,7 +216,7 @@ class UserDatabase {
         ensures userList[..] == users[..] && passList[..] == passwords[..]
     {
         userList := new int[users.Length];
-        passList := new string[passwords.Length];
+        passList := new string[passwords.Length]; 
         var i := 0;
         while i < users.Length
         decreases users.Length - i
@@ -166,6 +236,7 @@ method seqToArrInt(s: seq<int>) returns(a: array<int>)
     ensures a.Length == |s|
     ensures forall i :: 0 <= i < |s| ==> a[i] == s[i]
     ensures multiset(a[..]) == multiset(s)
+    ensures fresh(a)
 {
     a := new int[|s|];
     var i := 0;
@@ -185,6 +256,7 @@ method seqToArrStr(s: seq<string>) returns(a: array<string>)
     ensures a.Length == |s|
     ensures forall i :: 0 <= i < |s| ==> a[i] == s[i]
     ensures multiset(a[..]) == multiset(s)
+    ensures fresh(a)
 {
     a := new string[|s|];
     var i := 0;
@@ -205,4 +277,20 @@ function DualRange(a: array<int>, low: int, mid1: int, mid2: int, high: int): se
     requires 0 <= low <= mid1 <= mid2 <= high <= a.Length;
 {
     a[low..mid1] + a[mid2..high]
+}
+
+predicate LTRange(a: array<int>, low: int, high: int, key: int) 
+reads a; 
+requires a != null;
+requires 0 <= low <= high <= a.Length;
+{
+    forall j :: low <= j < high ==> a[j] < key
+}
+
+predicate GERange(a: array<int>, low: int, high: int, key: int)
+reads a;
+requires a != null;
+requires 0 <= low <= high <= a.Length;
+{
+    forall j :: low <= j < high ==> a[j] >= key
 }
